Aesop/DefaultRules.lean
@@ -26,18 +26,18 @@ end DefaultRules
 -- tag the above tactics with `@[aesop ... (rule_set default)]` or something.
 def defaultRules : TermElabM (Array RuleSetMember) := do
   mkRules #[
-    (``DefaultRules.safeAssumption , ← `(attr|aesop safe -50)),
+    (``DefaultRules.safeAssumption , ← `(attr|aesop safe -50   (builder tactic uses_no_branch_state))),
       -- The assumption rule is subsumed by applyHyps. But we still want to have
       -- it separately as a low-penalty safe rule so that very easy goals are
       -- discharged immediately.
-    (``DefaultRules.safeReflexivity, ← `(attr|aesop safe -49)),
-    (``DefaultRules.intros         , ← `(attr|aesop norm -1)),
-    (``DefaultRules.splitHyps      , ← `(attr|aesop norm 0)),
-    (``DefaultRules.applyHyps      , ← `(attr|aesop 75%))]
+    (``DefaultRules.safeReflexivity, ← `(attr|aesop safe -49   (builder tactic uses_no_branch_state))),
+    (``DefaultRules.intros         , ← `(attr|aesop norm -1    (builder tactic uses_no_branch_state))),
+    (``DefaultRules.splitHyps      , ← `(attr|aesop norm 0     (builder tactic uses_no_branch_state))),
+    (``DefaultRules.applyHyps      , ← `(attr|aesop unsafe 75% (builder tactic uses_no_branch_state)))]
   where
     mkRule (decl : Name) (configStx : Syntax) :
         TermElabM (Array RuleSetMember) := do
-      let config ← RuleConfig.parse configStx
+      let config ← Config.RuleConfig.parse configStx
       config.applyToRuleIdent (RuleIdent.const decl)
 
     mkRules (rs : Array (Name × Syntax)) : TermElabM (Array RuleSetMember) :=
