tests/BranchState.lean
@@ -2,19 +2,20 @@ import Aesop
 
 open Aesop
 
+set_option aesop.check.all true
+
 inductive Even : Nat → Prop
 | zero : Even 0
 | plusTwo : Even n → Even (n + 2)
 
 attribute [aesop safe] Even.zero
 
-@[aesop safe]
 def limitedEvenPlusTwo : RuleTac :=
   RuleTac.withApplicationLimit 2 $ RuleTac.applyConst ``Even.plusTwo
 
 example : Even 4 := by
-  aesop
+  aesop (safe [limitedEvenPlusTwo])
 
 example : Even 6 := by
-  fail_if_success aesop
-  exact Even.plusTwo $ Even.plusTwo $ Even.plusTwo Even.zero
+  fail_if_success aesop (safe [limitedEvenPlusTwo])
+  aesop (safe [limitedEvenPlusTwo (builder tactic uses_no_branch_state)])
